Add some corollaries

Wavelet/Simulation.lean
@@ -20,8 +20,10 @@ variable (Op : Type u) (χ : Type u) (V S)
 variable [instArity : Arity Op] [DecidableEq χ] [instInterp : Interp Op V S]
 
 /-- Main simulation theorem from `Fn` to compiled `Proc`. -/
-theorem sim_dataflow
-  {fn : Fn Op χ m n} {args : Vector V m} {state : S}
+theorem sim_compile_fn
+  (fn : Fn Op χ m n)
+  (args : Vector V m)
+  (state : S)
   (hnz : m > 0 ∧ n > 0)
   (hwf_fn : fn.WellFormed) :
   ∃ pc',
@@ -48,5 +50,78 @@ theorem sim_dataflow
         | tail => exact Simulation.Tail.sim_step_tail Op χ V S hnz ec ec' pc hsim hstep hcont
         | op => exact Simulation.Op.sim_step_op Op χ V S hnz ec ec' pc hsim hstep hcont
         | br => exact Simulation.Br.sim_step_br Op χ V S hnz ec ec' pc hsim hstep hcont
+
+/-- Converts a trace of `Seq` to a trace of `Dataflow` with
+related final configurations. -/
+theorem SeqRefinesDataflow_steps_to_steps
+  [DecidableEq χ₁] [DecidableEq χ₂]
+  (ec : Seq.Config Op χ₁ V S m n)
+  (pc : Dataflow.Config Op χ₂ V S m n)
+  (href : SeqRefinesDataflow Op V S ec pc R)
+  (hsteps : Seq.Config.StepStar Op χ₁ V S ec ec') :
+  ∃ pc',
+    Dataflow.Config.StepStar Op χ₂ V S pc pc' ∧
+    R ec' pc'
+:= by
+  induction hsteps with
+  | refl =>
+    exists pc
+    constructor
+    · exact .refl
+    · exact href.1
+  | tail hsteps_ec hstep_ec₁ ih =>
+    rename_i ec₁ ec₂
+    have ⟨pc₁, hsteps_pc, hr⟩ := ih
+    have ⟨pc₂, hsteps_pc₁, hr'⟩ := href.2 ec₁ pc₁ ec₂ hr hstep_ec₁
+    exists pc₂
+    have hsteps := Relation.ReflTransGen.trans hsteps_pc hsteps_pc₁.to_reflTransGen
+    simp [hr']
+    exact hsteps
+
+/-- Defines the final channel state with the given return values. -/
+def finalChans (retVals : Vector V n) : ChanMap (ChanName χ) V :=
+  λ name =>
+    match name with
+    | .final_dest i => if _ : i < n then [retVals[i]] else []
+    | _ => []
+
+/-- Same results at termination. -/
+theorem sim_compile_fn_forward_results
+  (fn : Fn Op χ m n)
+  (args : Vector V m)
+  (state : S)
+  (hnz : m > 0 ∧ n > 0)
+  (hwf_fn : fn.WellFormed)
+  (hsteps : Seq.Config.StepStar Op χ V S (Seq.Config.init _ _ _ _ fn state args) ec)
+  (hterm : ec.expr = .ret retVals) :
+  ∃ pc',
+    Dataflow.Config.StepStar Op (ChanName χ) V S
+      (Dataflow.Config.init _ _ _ _ (compileFn Op χ V S hnz fn) state args) pc' ∧
+    pc'.state = ec.state ∧
+    pc'.chans = finalChans _ _ retVals
+:= by
+  have ⟨pc', hsteps_pc, href⟩ :=
+    sim_compile_fn Op χ V S fn args state hnz hwf_fn
+  have ⟨pc₂, hsteps_pc', hsim⟩ := SeqRefinesDataflow_steps_to_steps _ _ _ _ pc' href hsteps
+  have ⟨heq_state, hchans, _, hdefined_vars, _, _, _, _, _, _, _,
+    _, _, _, _, _, hret, _⟩ := hsim
+  exists pc₂
+  and_intros
+  · exact Relation.ReflTransGen.trans hsteps_pc hsteps_pc'
+  · simp [heq_state]
+  · funext name
+    simp [hchans, SimR.varsToChans, finalChans]
+    have ⟨_, _, _, hdefined_vars_empty, hpath_conds_empty⟩ := hret _ hterm
+
+    cases name with
+    | var v pathConds =>
+      simp [hpath_conds_empty]
+      intros _
+      split <;> rename_i h₁
+      · have := (hdefined_vars v).mpr ⟨_, h₁⟩
+        simp [hdefined_vars_empty] at this
+      · rfl
+    | final_dest i => simp [hterm]
+    | _ => simp [hpath_conds_empty]
 
 end Wavelet.Simulation
